Update montred to newish pipeline, revive DCE
- Update the style of montred snythesis to match the changes in the
  pipeline
- Bring back non-quadratic dead code elimination and make use of it for
  montgomery reduction
- Update partial reduction to inline "var-like" things (fst, snd, pair
  applied to var)

src/Experiments/SimplyTypedArithmetic.v
@@ -3564,6 +3564,18 @@ Module Compilers.
     Module ident.
       Section interp.
         Context {var : type -> Type}.
+        Fixpoint is_var_like {t} (e : @expr var t) : bool
+          := match e with
+             | Var t v => true
+             | TT => true
+             | AppIdent _ _ (ident.fst _ _) args => @is_var_like _ args
+             | AppIdent _ _ (ident.snd _ _) args => @is_var_like _ args
+             | Pair A B a b => @is_var_like A a && @is_var_like B b
+             | AppIdent _ _ _ _ => false
+             | App _ _ _ _
+             | Abs _ _ _
+               => false
+             end.
         Fixpoint interp_let_in {tC tx : type} {struct tx} : value var tx -> (value var tx -> value var tC) -> value var tC
           := match tx return value var tx -> (value var tx -> value var tC) -> value var tC with
              | type.arrow _ _
@@ -3600,10 +3612,9 @@ Module Compilers.
                       (f : sign * expr t + type.interp t -> value var tC)
                   => match x with
                      | inl (sgn, e)
-                       => match invert_Var e with
-                          | Some v => f (inl (sgn, Var v))
-                          | None => partial.expr.reflect (expr_let y := e in partial.expr.reify (f (inl (sgn, Var y)%core)))%expr
-                          end
+                       => if is_var_like e
+                          then f (inl (sgn, e))
+                          else partial.expr.reflect (expr_let y := e in partial.expr.reify (f (inl (sgn, Var y)%core)))%expr
                      | inr v => f (inr v)
                      end
              | type.type_primitive _ as t
@@ -3966,6 +3977,104 @@ Module Compilers.
 
   Definition PartialReduce {t} (e : Expr t) : Expr t
     := fun var => @partial_reduce var t (e _).
+
+  Module DeadCodeElimination.
+    Fixpoint compute_live' {t} (e : @expr (fun _ => PositiveSet.t) t) (cur_idx : positive)
+    : positive * PositiveSet.t
+      := match e with
+         | Var t v => (cur_idx, v)
+         | TT => (cur_idx, PositiveSet.empty)
+         | AppIdent s d idc args
+           => let default := @compute_live' _ args cur_idx in
+              match args in expr.expr t return ident.ident t d -> _ with
+              | Pair A B x (Abs s d f)
+                => fun idc
+                   => match idc with
+                      | ident.Let_In _ _
+                        => let '(idx, live) := @compute_live' A x cur_idx in
+                           let '(_, live) := @compute_live' _ (f (PositiveSet.add idx live)) (Pos.succ idx) in
+                           (Pos.succ idx, live)
+                      | _ => default
+                      end
+              | _ => fun _ => default
+              end idc
+         | App s d f x
+           => let '(idx, live1) := @compute_live' _ f cur_idx in
+              let '(idx, live2) := @compute_live' _ x idx in
+              (idx, PositiveSet.union live1 live2)
+         | Pair A B a b
+           => let '(idx, live1) := @compute_live' A a cur_idx in
+              let '(idx, live2) := @compute_live' B b idx in
+              (idx, PositiveSet.union live1 live2)
+         | Abs s d f
+           => let '(_, live) := @compute_live' _ (f PositiveSet.empty) cur_idx in
+              (cur_idx, live)
+         end.
+    Definition compute_live {t} e : PositiveSet.t := snd (@compute_live' t e 1).
+    Definition ComputeLive {t} (e : Expr t) := compute_live (e _).
+
+    Section with_var.
+      Context {var : type -> Type}
+              (live : PositiveSet.t).
+      Definition OUGHT_TO_BE_UNUSED {T1 T2} (v : T1) (v' : T2) := v.
+      Global Opaque OUGHT_TO_BE_UNUSED.
+      Fixpoint eliminate_dead' {t} (e : @expr (@expr var) t) (cur_idx : positive)
+        : positive * @expr var t
+        := match e with
+           | Var t v => (cur_idx, v)
+           | TT => (cur_idx, TT)
+           | AppIdent s d idc args
+             => let default := @eliminate_dead' _ args cur_idx in
+                let default := (fst default, AppIdent idc (snd default)) in
+                match args in expr.expr t return ident.ident t d -> positive * expr d -> positive * expr d with
+                | Pair A B x y
+                  => match y in expr.expr Y return ident.ident (A * Y) d -> positive * expr d -> positive * expr d with
+                     | Abs s' d' f
+                       => fun idc
+                          => let '(idx, x') := @eliminate_dead' A x cur_idx in
+                             let f' := fun v => snd (@eliminate_dead' _ (f v) (Pos.succ idx)) in
+                             match idc in ident.ident s d
+                                   return (match s return Type with
+                                           | A * _ => expr A
+                                           | _ => unit
+                                           end%ctype
+                                           -> match s return Type with
+                                              | _ * (s -> d) => (expr s -> expr d)%type
+                                              | _ => unit
+                                              end%ctype
+                                           -> positive * expr d
+                                           -> positive * expr d)
+                             with
+                             | ident.Let_In _ _
+                               => fun x' f' _
+                                  => if PositiveSet.mem idx live
+                                     then (Pos.succ idx, AppIdent ident.Let_In (Pair x' (Abs (fun v => f' (Var v)))))
+                                     else (Pos.succ idx, f' (OUGHT_TO_BE_UNUSED x' (Pos.succ idx, PositiveSet.elements live)))
+                             | _ => fun _ _ default => default
+                             end x' f'
+                     | _ => fun _ default => default
+                     end
+                | _ => fun _ default => default
+                end idc default
+           | App s d f x
+             => let '(idx, f') := @eliminate_dead' _ f cur_idx in
+                let '(idx, x') := @eliminate_dead' _ x idx in
+                (idx, App f' x')
+           | Pair A B a b
+             => let '(idx, a') := @eliminate_dead' A a cur_idx in
+                let '(idx, b') := @eliminate_dead' B b idx in
+                (idx, Pair a' b')
+           | Abs s d f
+             => (cur_idx, Abs (fun v => snd (@eliminate_dead' _ (f (Var v)) cur_idx)))
+           end.
+
+      Definition eliminate_dead {t} e : expr t
+        := snd (@eliminate_dead' t e 1).
+    End with_var.
+
+    Definition EliminateDead {t} (e : Expr t) : Expr t
+      := fun var => eliminate_dead (ComputeLive e) (e _).
+  End DeadCodeElimination.
 
   Module ReassociateSmallConstants.
     Import Compilers.Uncurried.expr.default.
@@ -5347,8 +5456,11 @@ Ltac cache_reify _ :=
   end;
   [ repeat match goal with |- context[expr.Interp _ _ _] => apply (f_equal (fun f => f _)) end;
     apply f_equal;
-    time lazy;
-    reflexivity
+    lazymatch goal with |- ?LHS = ?RHS => subst LHS end;
+    let RHS := lazymatch goal with |- ?LHS = ?RHS => RHS end in
+    time (let RHS' := (eval vm_compute in RHS) in (* [vm_compute] is much faster than [lazy] here on large things *)
+          time instantiate (1:=RHS');
+          vm_cast_no_check (eq_refl RHS'))
   | clearbody E ].
 
 Derive carry_mul_gen
@@ -5505,6 +5617,7 @@ Module Pipeline.
        end.
 
   Definition BoundsPipeline
+             (with_dead_code_elimination : bool)
              relax_zrange
              {s d}
              arg_bounds
@@ -5512,6 +5625,7 @@ Module Pipeline.
              (E : Expr (s -> d))
   : ErrorT (BoundsAnalysis.Indexed.expr.Notations.expr (BoundsAnalysis.Indexed.Range.type_for_range relax_zrange (t:=BoundsAnalysis.Indexed.OfPHOAS.type.compile d) out_bounds))
     := let E := PartialReduce E in
+       let E := if with_dead_code_elimination then DeadCodeElimination.EliminateDead E else E in
        let E := ReassociateSmallConstants.Reassociate (2^8) E in
        let E := BoundsAnalysis.OfPHOAS.AnalyzeBounds relax_zrange E arg_bounds in
        let E := match E with
@@ -5524,13 +5638,14 @@ Module Pipeline.
        E.
 
   Lemma BoundsPipeline_correct
+             (with_dead_code_elimination : bool)
              relax_zrange
              {s d}
              arg_bounds
              out_bounds
              (E : Expr (s -> d))
              rv
-             (Hrv : BoundsPipeline relax_zrange arg_bounds out_bounds E = Success rv)
+             (Hrv : BoundsPipeline with_dead_code_elimination relax_zrange arg_bounds out_bounds E = Success rv)
     : forall arg
              (Harg : BoundsAnalysis.Indexed.Range.type_for_range_bounded_by
                        relax_zrange
@@ -5554,12 +5669,14 @@ Module Pipeline.
   Admitted.
 
   Definition BoundsPipelineConst
+             (with_dead_code_elimination : bool)
              relax_zrange
              {t}
              bounds
              (E : Expr t)
   : ErrorT (BoundsAnalysis.Indexed.expr.Notations.expr (BoundsAnalysis.Indexed.Range.type_for_range relax_zrange (t:=BoundsAnalysis.Indexed.OfPHOAS.type.compile t) bounds))
     := let E := PartialReduce E in
+       let E := if with_dead_code_elimination then DeadCodeElimination.EliminateDead E else E in
        let E := ReassociateSmallConstants.Reassociate (2^8) E in
        let E := BoundsAnalysis.OfPHOAS.AnalyzeBoundsConst relax_zrange E in
        let E := match E with
@@ -5572,12 +5689,13 @@ Module Pipeline.
        E.
 
   Lemma BoundsPipelineConst_correct
+             (with_dead_code_elimination : bool)
              relax_zrange
              {d}
              bounds
              (E : Expr d)
              rv
-             (Hrv : BoundsPipelineConst relax_zrange bounds E = Success rv)
+             (Hrv : BoundsPipelineConst with_dead_code_elimination relax_zrange bounds E = Success rv)
     : exists res,
         let ctx := PositiveMap.empty _ in
         BoundsAnalysis.Indexed.expr.interp (@BoundsAnalysis.ident.interp) rv ctx
@@ -5749,6 +5867,7 @@ Section rcarry_mul.
 
   Let BoundsPipeline21 in_bounds out_bounds res
     := let res := Pipeline.BoundsPipeline
+                    false
                     relax_zrange
                     (s:=(type.list type.Z * type.list type.Z)%ctype)
                     (d:=(type.list type.Z)%ctype)
@@ -5759,6 +5878,7 @@ Section rcarry_mul.
 
   Let BoundsPipeline11 in_bounds out_bounds res
     := let res := Pipeline.BoundsPipeline
+                    false
                     relax_zrange
                     (s:=(type.list type.Z)%ctype)
                     (d:=(type.list type.Z)%ctype)
@@ -5768,9 +5888,11 @@ Section rcarry_mul.
        res.
 
   Definition rexpr_1_correctT_ctx
+             relax_zrange
+             t_out
              ctx
              out_bounds
-             (f : type.interp (type.list type.Z))
+             (f : type.interp t_out)
              rv
     := (exists res,
            BoundsAnalysis.Indexed.expr.interp (@BoundsAnalysis.ident.interp) rv ctx
@@ -5781,9 +5903,10 @@ Section rcarry_mul.
               = f).
 
   Definition rexpr_n1_correctT
-             t_in
+             relax_zrange
+             t_in t_out
              in_bounds out_bounds
-             (f : _ -> type.interp (type.list type.Z))
+             (f : _ -> type.interp t_out)
              rv
     := forall arg
               (arg' := @BoundsAnalysis.OfPHOAS.cast_back
@@ -5798,34 +5921,38 @@ Section rcarry_mul.
       let ctx :=
           BoundsAnalysis.Indexed.Context.extendb
             (PositiveMap.empty _) 1 arg in
-      @rexpr_1_correctT_ctx ctx out_bounds (f arg') rv.
+      @rexpr_1_correctT_ctx relax_zrange t_out ctx out_bounds (f arg') rv.
 
   Definition rexpr_21_correctT
              in_bounds out_bounds
              (f : _ -> type.interp (type.list type.Z))
              rv
-    := @rexpr_n1_correctT (type.list type.Z * type.list type.Z)
+    := @rexpr_n1_correctT relax_zrange
+                          (type.list type.Z * type.list type.Z)
+                          (type.list type.Z)
                           (in_bounds, in_bounds) out_bounds f rv.
 
   Definition rexpr_11_correctT
              in_bounds out_bounds
              (f : _ -> type.interp (type.list type.Z))
              rv
-    := @rexpr_n1_correctT (type.list type.Z)
+    := @rexpr_n1_correctT relax_zrange
+                          (type.list type.Z)
+                          (type.list type.Z)
                           in_bounds out_bounds f rv.
 
   Definition rexpr_Z1_correctT
              in_bounds out_bounds
              (f : _ -> type.interp (type.list type.Z))
              rv
-    := @rexpr_n1_correctT type.Z
+    := @rexpr_n1_correctT relax_zrange type.Z (type.list type.Z)
                           in_bounds out_bounds f rv.
 
   Definition rexpr_01_correctT
              out_bounds
              (f : type.interp (type.list type.Z))
              rv
-    := @rexpr_1_correctT_ctx (PositiveMap.empty _) out_bounds f rv.
+    := @rexpr_1_correctT_ctx relax_zrange (type.list type.Z) (PositiveMap.empty _) out_bounds f rv.
 
   Definition rcarry_mul
     := let res := BoundsPipeline21
@@ -5858,6 +5985,7 @@ Section rcarry_mul.
 
   Definition rcarry
     := let res := Pipeline.BoundsPipeline
+                    false
                     relax_zrange
                     (s:=(type.list type.Z)%ctype)
                     (d:=(type.list type.Z)%ctype)
@@ -5890,6 +6018,7 @@ Section rcarry_mul.
 
   Definition rrelax
     := let res := Pipeline.BoundsPipeline
+                    false
                     relax_zrange
                     (s:=(type.list type.Z)%ctype)
                     (d:=(type.list type.Z)%ctype)
@@ -5996,6 +6125,7 @@ Section rcarry_mul.
 
   Definition rencode
     := let res := Pipeline.BoundsPipeline
+                    false
                     relax_zrange
                     (s:=type.Z)
                     (d:=(type.list type.Z)%ctype)
@@ -6026,6 +6156,7 @@ Section rcarry_mul.
 
   Definition rzero
     := let res := Pipeline.BoundsPipelineConst
+                    false
                     relax_zrange
                     (t:=(type.list type.Z)%ctype)
                     tight_bounds
@@ -6054,6 +6185,7 @@ Section rcarry_mul.
 
   Definition rone
     := let res := Pipeline.BoundsPipelineConst
+                    false
                     relax_zrange
                     (t:=(type.list type.Z)%ctype)
                     tight_bounds
@@ -6281,7 +6413,7 @@ Section rcarry_mul.
                => cbv [tight_bounds loose_bounds] in H |- *; rewrite H
              | _ => rewrite BoundsAnalysis.OfPHOAS.cast_back_primitive_cast_primitive in *
              | [ fx := (BoundsAnalysis.Indexed.expr.interp _ ?rop (BoundsAnalysis.Indexed.Context.extendb _ _ ?x)),
-                       H : forall arg, BoundsAnalysis.Indexed.Range.type_for_range_bounded_by _ ?bs arg = true -> rexpr_1_correctT_ctx _ _ _ ?rop
+                       H : forall arg, BoundsAnalysis.Indexed.Range.type_for_range_bounded_by _ ?bs arg = true -> rexpr_1_correctT_ctx _ _ _ _ _ ?rop
                                        |- _ ]
                => destruct (H x); [ clear H | subst fx ]
              | [ fx := Option.bind ?x ?f, H : ?x = Some ?v |- _ ]
@@ -6291,9 +6423,6 @@ Section rcarry_mul.
                   assert (H' : fx = fx')
                     by (subst fx fx'; apply f_equal2; [ exact H | reflexivity ]);
                   cbn [Option.bind] in fx'; clearbody fx; subst fx
-             (*| [ H : forall arg, BoundsAnalysis.Indexed.Range.type_for_range_bounded_by _ ?bs arg = true -> rexpr_1_correctT_ctx _ _ _ ?rop
-                                 |- context[BoundsAnalysis.Indexed.expr.interp _ ?rop (BoundsAnalysis.Indexed.Context.extendb _ _ ?x)] ]
-               => specialize (H x); destruct H*)
              | _ => progress cbn [BoundsAnalysis.OfPHOAS.cast_back] in * (* for getting eauto to work *)
              end.
 
@@ -6574,6 +6703,7 @@ Module PrintingNotations.
   Export BoundsAnalysis.ident.
   Export BoundsAnalysis.Notations.
   Open Scope btype_scope.
+  Global Set Printing Width 100000.
   Notation "'uint256'"
     := (r[0 ~> 115792089237316195423570985008687907853269984665640564039457584007913129639935]%btype) : btype_scope.
   Notation "'uint128'"
@@ -6950,71 +7080,6 @@ Module X25519_32.
 End X25519_32.
 *)
 
-Module RemoveDeadLets.
-  Import BoundsAnalysis.Indexed.expr.
-  Section RemoveDeadLets.
-    Local Notation ident := BoundsAnalysis.ident.ident.
-
-    Fixpoint let_used (t : BoundsAnalysis.type.type) (n : positive)
-             (e : @expr ident t) : bool :=
-      match e with
-      | Var T m => Pos.eqb n m
-      | TT => false
-      | AppIdent s _ _ x => let_used s n x
-      | Pair A B a b => (let_used A n a) || (let_used B n b)
-      | Let_In s d m x f =>
-        (negb (Pos.eqb n m && negb (let_used s n x))) && ((let_used s n x) || (let_used d n f))
-      end.
-
-    Fixpoint remove_dead_lets (t : BoundsAnalysis.type.type) (e : @expr ident t) : @expr ident t :=
-      match e in (expr t') return expr t' with
-      | Var T n => Var T n
-      | TT => TT
-      | AppIdent s T idc x =>
-        AppIdent idc (remove_dead_lets _ x)
-      | Pair A B a b => Pair (remove_dead_lets _ a) (remove_dead_lets _ b)
-      | Let_In s T n x f =>
-        if (let_used T n f)
-        then Let_In n (remove_dead_lets _ x) (remove_dead_lets _ f)
-        else remove_dead_lets _ f
-      end.
-
-    Fixpoint inline_let (idx : positive) Tnew (new : @expr ident Tnew) t (e : @expr ident t) : @expr ident t :=
-      match e in expr t' return expr t' with
-      | Var T n => if (Pos.eqb n idx)
-                   then match BoundsAnalysis.type.transport (@expr ident) Tnew T new with
-                        | Some new' => new'
-                        | None => Var T n
-                        end
-                   else Var T n
-      | TT => TT
-      | AppIdent s T idc x => AppIdent idc (inline_let idx _ new _ x)
-      | Pair A B a b => Pair (inline_let idx _ new _ a) (inline_let idx _ new _ b)
-      | Let_In s T n x f => Let_In n (inline_let idx _ new _ x) (inline_let idx _ new _ f)
-      end.
-
-    (* inlines lets that just re-bind a variable or half a variable with type prod *)
-    Fixpoint inline_silly_lets t (e : @expr ident t) : @expr ident t :=
-      match e in (expr t') return expr t' with
-      | Var T n => Var T n
-      | TT => TT
-      | AppIdent s T idc x =>
-        AppIdent idc (inline_silly_lets _ x)
-      | Pair A B a b => Pair (inline_silly_lets _ a) (inline_silly_lets _ b)
-      | Let_In s T n x f =>
-        match x with
-        | Var T' m => inline_let n _ (Var T' m) _ f
-        | AppIdent _ _ (@BoundsAnalysis.ident.fst A B) (Var _ m) =>
-          inline_let n _ (@AppIdent _ _ _ (@BoundsAnalysis.ident.fst A B) (Var _ m)) _ (inline_silly_lets _ f)
-        | _ => Let_In n (inline_silly_lets _ x) (inline_silly_lets _ f)
-        end
-      end.
-
-    (* TODO: proofs--note these may block on getting canonical maps for contexts *)
-    (* TODO(jgross, from jadep): Should I put this into the pipeline? *)
-  End RemoveDeadLets.
-End RemoveDeadLets.
-
 Require Import Crypto.Arithmetic.MontgomeryReduction.Definition.
 Require Import Crypto.Arithmetic.MontgomeryReduction.Proofs.
 Require Import Crypto.Util.ZUtil.EquivModulo.
@@ -7126,30 +7191,7 @@ Module MontgomeryReduction.
                              montred_gen N R N' w w_half n lo_hi
                       = montred' N R N' w w_half n lo_hi)
          As montred_gen_correct.
-  Proof.
-    intros.
-    etransitivity.
-    Focus 2.
-    { repeat apply (f_equal (fun f => f _)).
-      Reify_rhs().
-      reflexivity. } Unfocus.
-    cbv beta.
-    let RHS := match goal with |- _ = ?RHS => RHS end in
-    let e := match RHS with context[expr.Interp _ ?e] => e end in
-    set (E := e).
-    Time let E' := constr:(PartialReduce (CPS.CallFunWithIdContinuation (CPS.Translate (canonicalize_list_recursion E)))) in
-         let E' := (eval vm_compute in E') in (* 0.131 for vm, about 0.6 for lazy, slower for native and cbv *)
-         pose E' as E''.
-    let LHS := match goal with |- ?LHS = _ => LHS end in
-    lazymatch LHS with
-    | context LHS[expr.Interp _ _]
-      => let LHS := context LHS[Interp E''] in
-         transitivity LHS
-    end;
-      [ clear E | exact admit ].
-    subst montred_gen.
-    reflexivity.
-  Qed.
+  Proof. Time cache_reify (). exact admit. (* correctness of initial parts of the pipeline *) Time Qed.
 
   Section rmontred.
     Context (N R N' : Z)
@@ -7191,6 +7233,7 @@ Module MontgomeryReduction.
 
     Definition rmontred
       := let res := Pipeline.BoundsPipeline
+                      true
                       (relax_zrange)
                       (s:=(type.Z * type.Z)%ctype)
                       (d:=(type.Z)%ctype)
@@ -7205,44 +7248,48 @@ Module MontgomeryReduction.
                             @ (rw_half _)
                             @ (rn _)
                       )%expr in
-         check_args res.
+         res.
+
+    (* copied from above *)
+    Local Ltac solve_correct_gen pipeline_lem gen_correct :=
+      let Hrv := lazymatch goal with H : ?rop = Pipeline.Success _ |- _ => H end in
+      let rop := lazymatch type of Hrv with ?rop = Pipeline.Success _ => rop end in
+      hnf; intros; cbv [rop] in Hrv;
+      eapply pipeline_lem in Hrv; [ | eassumption.. ];
+      let res := fresh "res" in
+      destruct Hrv as [res Hrv];
+      exists res; do 2 try apply conj;
+      [ | | etransitivity ];
+      [ solve [ apply Hrv ].. | ];
+      repeat match goal with H := _ |- _ => subst H end;
+      erewrite <- gen_correct;
+      cbv [expr.Interp];
+      cbn [expr.interp];
+      f_equal;
+      cbn -[reify_list];
+      try (rewrite interp_reify_list, map_map; cbn;
+           erewrite map_ext with (g:=id), map_id; try reflexivity);
+      try (intros []; reflexivity).
+    Local Ltac solve_correct gen_correct :=
+      solve_correct_gen Pipeline.BoundsPipeline_correct gen_correct.
+    Local Ltac solve_correct_const gen_correct :=
+      solve_correct_gen Pipeline.BoundsPipelineConst_correct gen_correct.
 
     Definition rmontred_correctT
                rv
-      := forall arg
-                (arg' := @BoundsAnalysis.OfPHOAS.cast_back
-                           _
-                           (relax_zrange)
-                           (arg_bounds)
-                           arg),
-        BoundsAnalysis.OfPHOAS.Interp
-          (relax_zrange)
-          (arg_bounds)
-          (bs:=out_bounds)
-          arg
-          rv
-        = Some (montred' (Interp rN) (Interp rR) (Interp rN') (Interp rw) (Interp rw_half) (Interp rn) arg').
+      := Eval hnf in
+          @rexpr_n1_correctT
+            relax_zrange
+            ((type.Z * type.Z)%ctype) type.Z
+            arg_bounds out_bounds
+            (montred' (Interp rN) (Interp rR) (Interp rN') (Interp rw) (Interp rw_half) (Interp rn))
+            rv.
 
     Lemma rmontred_correct
           rv
           (Hrv : rmontred = Pipeline.Success rv)
       : rmontred_correctT rv.
-    Proof.
-      hnf; intros.
-      cbv [rmontred] in Hrv.
-      edestruct (Pipeline.BoundsPipeline _ _ _ _) as [rv'|] eqn:Hrv';
-        [ | clear -Hrv; cbv [check_args] in Hrv; break_innermost_match_hyps; discriminate ].
-      erewrite <- montred_gen_correct.
-      eapply Pipeline.BoundsPipeline_correct in Hrv'.
-      apply check_args_success_id in Hrv; inversion Hrv; subst rv.
-      rewrite Hrv'.
-      cbv [expr.Interp].
-      cbn [expr.interp].
-      apply f_equal; f_equal;
-        cbn -[reify_list];
-        rewrite interp_reify_list, map_map; cbn;
-          erewrite map_ext with (g:=id), map_id; try reflexivity.
-    Qed.
+    Proof. solve_correct montred_gen_correct. Qed.
   End rmontred.
 End MontgomeryReduction.
 
@@ -7257,25 +7304,14 @@ Module Montgomery256.
   Definition R := (2^256).
   Definition machine_wordsize := 256.
 
-  Derive montred256_with_dead_code
-         SuchThat (MontgomeryReduction.rmontred_correctT N R N' machine_wordsize montred256_with_dead_code)
+  Derive montred256
+         SuchThat (MontgomeryReduction.rmontred_correctT N R N' machine_wordsize montred256)
          As montred256_correct.
   Proof. Time solve_rmontred(). Time Qed.
 
-  (* TODO: if dead code calls dead code, then remove_dead_lets can
-  progress if called multiple times. Should probably fix this, but
-  termination of fixpoints is hard *)
-  Definition montred256 := Eval lazy in
-        (RemoveDeadLets.remove_dead_lets _
-        (RemoveDeadLets.remove_dead_lets _
-        (RemoveDeadLets.remove_dead_lets _
-        (RemoveDeadLets.remove_dead_lets _
-        (RemoveDeadLets.remove_dead_lets _
-        (RemoveDeadLets.remove_dead_lets _
-        (RemoveDeadLets.inline_silly_lets _ montred256_with_dead_code))))))).
-
   Import PrintingNotations.
   Open Scope nexpr_scope.
+  Set Printing Width 100000.
   Print montred256.
   (*
     expr_let 3 := (uint128)(fst @@ x_1 >> 128) in
